CpcMini/Lemmas.lean
@@ -39,36 +39,3 @@ theorem correct___eo_prog_symm (M : SmtModel) (x1 : Term) :
 by
   sorry
 
-
-
-
-/- Helper definitions -/
-
-def __eo_lem_state_to_formula_step : CStateObj -> Term -> Term
-  | CStateObj.assume F,
-      (Term.Apply (Term.Apply Term.imp F1) (Term.Apply (Term.Apply Term.imp F2) F3)) =>
-      (Term.Apply (Term.Apply Term.imp (Term.Apply (Term.Apply Term.and F) F1))
-        (Term.Apply (Term.Apply Term.imp F2) F3))
-  | CStateObj.assume_push F,
-      (Term.Apply (Term.Apply Term.imp F1) (Term.Apply (Term.Apply Term.imp F2) F3)) =>
-      (Term.Apply (Term.Apply Term.imp F1)
-        (Term.Apply (Term.Apply Term.imp (Term.Apply (Term.Apply Term.and F) F2)) F3))
-  | CStateObj.proven F,
-      (Term.Apply (Term.Apply Term.imp F1) (Term.Apply (Term.Apply Term.imp F2) F3)) =>
-      (Term.Apply (Term.Apply Term.imp F1)
-        (Term.Apply (Term.Apply Term.imp F2) (Term.Apply (Term.Apply Term.and F) F3)))
-  | _, _ => Term.Stuck
-
-
-def __eo_lem_state_to_formula_rec : CState -> Term -> Term
-  | _ , Term.Stuck  => Term.Stuck
-  | CState.nil, F => F
-  | (CState.cons so s), F => (__eo_lem_state_to_formula_step so (__eo_lem_state_to_formula_rec s F))
-  | CState.Stuck, F => Term.Stuck
-
-
-def __eo_lem_state_to_formula (s : CState) : Term :=
-  
-    let _v0 := (Term.Apply Term.imp (Term.Boolean true))
-    (__eo_lem_state_to_formula_rec s (Term.Apply _v0 (Term.Apply _v0 (Term.Boolean true))))
-
